avx2 safety proofs almost done

proof/safety/1024/avx2/safety_mlkem1024_avx2.ec
@@ -1091,7 +1091,6 @@ module Syscall : Syscall_t = {
   }
 }.
 
-
 module M(SC:Syscall_t) = {
   var tmp__trace : trace
   proc __shuffle8 (a:W256.t, b:W256.t) : W256.t * W256.t * trace = {
@@ -30612,7 +30611,7 @@ module M(SC:Syscall_t) = {
     (trace__shake256x4_A128__A32_A1 ++
     [(Assert,
      ((BArray800.is_init b_result_4 0 800) /\
-     (result_2 = ((param_11 + 1) + ((param_6 <> 0) ? 1 : 0)))))]);
+     (result_2 = (((param_11 + 1) %% param_5) + ((param_6 <> 0) ? 1 : 0)))))]);
     st <- result_3;
     param_18 <- st;
     b_param_2 <- b_out0;
@@ -30776,7 +30775,7 @@ module M(SC:Syscall_t) = {
     (trace__shake128x4_absorb_A32_A2 ++
     [(Assert,
      ((BArray800.is_init b_result 0 800) /\
-     (result_2 = ((param_11 + 2) + ((param_6 <> 0) ? 1 : 0)))))]);
+     (result_2 = (((param_11 + 2) %% param_5) + ((param_6 <> 0) ? 1 : 0)))))]);
     st <- result_3;
     b_st <- (BArray800.init_arr (W8.of_int 255));
     return (st, b_st, trace__shake128x4_absorb_A32_A2);
@@ -36310,18 +36309,7 @@ module M(SC:Syscall_t) = {
     trace___gen_matrix_buf_rejection_filter24 <-
     (trace___gen_matrix_buf_rejection_filter24 ++
     [(Assert,
-     (BArray512.is_init b_result_0 0
-     ((2 * (W64.to_uint param_1)) +
-     ((((16 < (2 * (256 - (W64.to_uint param_1)))) ? 16 : (2 *
-                                                          (256 -
-                                                          (W64.to_uint
-                                                          param_1)))) <
-      0) ? 0 : ((16 < (2 * (256 - (W64.to_uint param_1)))) ? 16 : (2 *
-                                                                  (256 -
-                                                                  (
-                                                                  W64.to_uint
-                                                                  param_1))))))
-     ))]);
+     (BArray512.is_init b_result_0 0 ((2 * (W64.to_uint param_1)) + 16)))]);
     b_pol <- b_result_0;
     pol <- result_0;
     ms <- result;
@@ -36341,18 +36329,7 @@ module M(SC:Syscall_t) = {
     trace___gen_matrix_buf_rejection_filter24 <-
     (trace___gen_matrix_buf_rejection_filter24 ++
     [(Assert,
-     (BArray512.is_init b_result 0
-     ((2 * (W64.to_uint param_5)) +
-     ((((16 < (2 * (256 - (W64.to_uint param_5)))) ? 16 : (2 *
-                                                          (256 -
-                                                          (W64.to_uint
-                                                          param_5)))) <
-      0) ? 0 : ((16 < (2 * (256 - (W64.to_uint param_5)))) ? 16 : (2 *
-                                                                  (256 -
-                                                                  (
-                                                                  W64.to_uint
-                                                                  param_5))))))
-     ))]);
+     (BArray512.is_init b_result 0 ((2 * (W64.to_uint param_5)) + 16)))]);
     b_pol <- b_result;
     pol <- result_2;
     ms <- result_1;
@@ -36618,7 +36595,7 @@ module M(SC:Syscall_t) = {
     (trace___gen_matrix_fill_polynomial ++
     [(Assert,
      (((W64.of_int (W64.to_uint param_1)) \ule result) /\
-     (BArray512.is_init b_param_0 0 (2 * (W64.to_uint result)))))]);
+     (BArray512.is_init b_result_1 0 (2 * (W64.to_uint result)))))]);
     b_pol <- b_result_1;
     pol <- result_0;
     counter <- result;
@@ -36650,7 +36627,7 @@ module M(SC:Syscall_t) = {
       (trace___gen_matrix_fill_polynomial ++
       [(Assert,
        (((W64.of_int (W64.to_uint param_6)) \ule result_2) /\
-       (BArray512.is_init b_param 0 (2 * (W64.to_uint result_2)))))]);
+       (BArray512.is_init b_result 0 (2 * (W64.to_uint result_2)))))]);
       b_pol <- b_result;
       pol <- result_3;
       counter <- result_2;
@@ -40194,8 +40171,9 @@ op a1____absorb_avx2x4_spec _st _b_st _aT _buf0 _b_buf0 _buf1 _b_buf1 _buf2 _b_b
    ((true /\
     (true /\
     (true /\
+    (true /\
     ((BArray800.is_init res.`2 0 (25 * 32)) /\
-    (res.`3 = ((_aT + 1) + ((__TRAILB <> 0) ? 1 : 0))))))) /\
+    (res.`3 = (((_aT + 1) %% __RATE8) + ((__TRAILB <> 0) ? 1 : 0)))))))) /\
    (valid res.`4))].
 
 op a2____a_ilen_read_upto8_at_spec _buf _b_buf _offset _dELTA _lEN _tRAIL _cUR _aT =
@@ -40469,8 +40447,9 @@ op a2____absorb_avx2x4_spec _st _b_st _aT _buf0 _b_buf0 _buf1 _b_buf1 _buf2 _b_b
    ((true /\
     (true /\
     (true /\
+    (true /\
     ((BArray800.is_init res.`2 0 (25 * 32)) /\
-    (res.`3 = ((_aT + 2) + ((__TRAILB <> 0) ? 1 : 0))))))) /\
+    (res.`3 = (((_aT + 2) %% __RATE8) + ((__TRAILB <> 0) ? 1 : 0)))))))) /\
    (valid res.`4))].
 
 op a32____a_ilen_read_upto8_at_spec _buf _b_buf _offset _dELTA _lEN _tRAIL _cUR _aT =
@@ -45682,21 +45661,7 @@ op __write_u128_boundchk_spec _pol _b_pol _ctr _data _ms =
    (((_ms = ms) /\
     ((_data = data) /\ ((_ctr = ctr) /\ ((_b_pol = b_pol) /\ (_pol = pol))))) /\
    (true /\ (BArray512.is_init _b_pol 0 (2 * (W64.to_uint _ctr))))) ==>
-   ((true /\
-    (true /\
-    (true /\
-    (true /\
-    (true /\
-    (BArray512.is_init res.`2 0
-    ((2 * (W64.to_uint _ctr)) +
-    ((((16 < (2 * (256 - (W64.to_uint _ctr)))) ? 16 : (2 *
-                                                      (256 -
-                                                      (W64.to_uint _ctr)))) <
-     0) ? 0 : ((16 < (2 * (256 - (W64.to_uint _ctr)))) ? 16 : (2 *
-                                                              (256 -
-                                                              (W64.to_uint
-                                                              _ctr))))))
-    )))))) /\
+   ((true /\ (BArray512.is_init res.`2 0 ((2 * (W64.to_uint _ctr)) + 16))) /\
    (valid res.`4))].
 
 op __gen_matrix_buf_rejection_filter24_spec _pol _b_pol _counter _buf _b_buf _buf_offset _load_shuffle _mask _bounds _sst _b_sst _ones _ms =
